WIP: Prove some more, generalize apply_all_once to all_once

coq/def/TODO.v
@@ -146,43 +146,47 @@ Definition insert_at (A:Type) (idx:nat) (x:A) (l:list A): list A :=
 
 (* Print sflib. There are several same definitions, __mark__, __guard__, etc.
 I intentionally define this new definition, not to mess these other things *)
-Definition __aa_mark__ A (a : A) : A := a.
+Definition __ao_mark__ A (a : A) : A := a.
 
-Lemma _aa_mark {A} (a: A) : __aa_mark__ A.
+Lemma _ao_mark {A} (a: A) : __ao_mark__ A.
 Proof. ss. Qed.
 
-Lemma _aa_unmark {A} (a: __aa_mark__ A) : A.
+Lemma _aa_unmark {A} (a: __ao_mark__ A) : A.
 Proof. ss. Qed.
 
 (* Made tactic applying @jeehoonkang's opinion *)
-Ltac aa_mark H := apply _aa_mark in H.
+Ltac ao_mark H := apply _ao_mark in H.
 Ltac aa_unmark H := apply _aa_unmark in H.
 
-(* Find one without __aa_mark__, and try applying "x".
-Regardless of success or fail, __aa_mark__ that.
+(* Find one without __ao_mark__, and try applying "x".
+Regardless of success or fail, __ao_mark__ that.
 By the nature of Ltac's match, it searches until it succeeds.
-If one success happen, _apply_all ends, so "repeat" in apply_all is needed.
-If all fails, "repeat" in apply_all will end, and will unmark all __aa_mark__.
+If one success happen, _all_once ends, so "repeat" in all_once is needed.
+If all fails, "repeat" in all_once will end, and will unmark all __ao_mark__.
 About repeat: https://coq.inria.fr/refman/Reference-Manual011.html#hevea_tactic201
  *)
-Ltac _apply_all x :=
+Tactic Notation "_all_once" tactic(tac) :=
   match goal with
   | [ H: ?y |- _ ] =>
     match y with
-    | (__aa_mark__ _) => fail 1
+    | (__ao_mark__ _) => fail 1
     | _ =>
-      try apply x in H; aa_mark H
+      try (tac H); ao_mark H
     end
   end.
 
 Ltac aa_unmark_all :=
   repeat match goal with
-  | [ H: (__aa_mark__ ?y) |- _ ] =>
+  | [ H: (__ao_mark__ ?y) |- _ ] =>
     aa_unmark H
   end.
 
-Ltac apply_all x :=
-  repeat (_apply_all x); aa_unmark_all.
+Tactic Notation "all_once" tactic(tac) :=
+  repeat (_all_once tac); aa_unmark_all.
+
+Ltac apply_in x H := apply x in H.
+
+Ltac apply_all_once x := all_once (apply_in x).
 
 Goal forall (a b c d e: bool) f,
     (negb true = false) -> (* IT SHOULD NOT RUN INF LOOP *)
@@ -197,12 +201,15 @@ Goal forall (a b c d e: bool) f,
     (negb (true && false) = true) -> False.
 Proof.
   i.
-  repeat (_apply_all negb_true_iff). (* all Prop should be __aa_mark__ed, regardless of success or fail *)
-  aa_unmark_all. (* all __aa_mark__ will disappear *)
+  repeat (_all_once (apply_in negb_true_iff)). (* all Prop should be __ao_mark__ed, regardless of success or fail *)
+  aa_unmark_all. (* all __ao_mark__ will disappear *)
   Undo. Undo.
-  Time apply_all negb_true_iff.
+  (* apply_in negb_true_iff H2. *)
+  Time all_once (apply_in negb_true_iff).
   Undo.
-  aa_mark H0. (* This will prevent apply_all to happen here *)
-  apply_all negb_true_iff.
-  (* User only needs to know "apply_all" and "aa_mark". *)
+  ao_mark H0. (* This will prevent all_once to happen here *)
+  all_once (apply_in negb_true_iff).
+  (* User only needs to know "all_once" and "ao_mark". *)
+  Undo. Undo.
+  apply_all_once negb_true_iff.
 Abort.
